Day 24: Verify decompiler, specify solve and solve2

src/aoc24.v
@@ -1,5 +1,5 @@
 From Coq Require Export ZArith.
-From stdpp Require Import gmap.
+From stdpp Require Import gmap lexico.
 
 Set Implicit Arguments.
 
@@ -19,7 +19,7 @@ Record instr := Mk_instr
   }.
 
 Notation "'input' a1 .. an" := (cons a1 .. (cons an nil) ..)
-  (at level 200, a1 custom alu, an custom alu).
+  (at level 200, a1 custom alu, an custom alu, only parsing).
 
 Notation "'add' r1 r2" := (Mk_instr Add r1%Z r2%Z)
   (in custom alu at level 1, r1 constr at level 0, r2 constr at level 0).
@@ -88,10 +88,11 @@ Fixpoint recognize (xs : list instr) : option (list (Z * Z * Z)) :=
 
 End Syntax.
 
-Definition step '((div_z, add_x, add_y) : Z * Z * Z) (rw : Z) (rz : Z) : Z :=
-  let rx := (rz mod 26) + add_x in
-  let rz := rz / div_z in
-  if rw =? rx then rz else rz * 26 + rw + add_y.
+Definition step '((div_z, add_x, add_y) : Z * Z * Z) (rw : Z) (rz : Z) : option Z :=
+  if (rz <? 0) || (div_z =? 0) then None else Some
+  ( let rx := (rz mod 26) + add_x in
+    let rz := Z.quot rz div_z in
+    if rx =? rw then rz else rz * 26 + rw + add_y).
 
 (* Recursion and memoization *)
 
@@ -191,23 +192,26 @@ Fixpoint log_lt (n : nat) (b k : Z) : bool :=
   end.
 
 Definition _search {M} `{Monad M} (digits : list Z)
-  : endo (Z * N -> list (Z -> Z -> Z) -> M (option (list Z))) := fun _search '(rz, n) ts =>
+  : endo (Z * N -> list (Z -> Z -> option Z) -> M (option (list Z))) := fun _search '(rz, n) ts =>
   match ts with
   | nil => if rz =? 0 then ret (Some nil) else ret None
   | t :: ts =>
     let?* d := digits in
-    let rz := t d rz in
-    if log_lt (13 - N.to_nat n) 26 rz then
-      let* r := _search (rz, N.succ n) ts in
-      ret (option_map (cons d) r)
-    else
-      ret None
+    match t d rz with
+    | None => ret None
+    | Some rz =>
+      if log_lt (13 - N.to_nat n) 26 rz then
+        let* r := _search (rz, N.succ n) ts in
+        ret (option_map (cons d) r)
+      else
+        ret None
+    end
   end.
 
 Definition decimal (xs : list Z) : Z :=
   fold_left (fun acc d => acc * 10 + d) xs 0.
 
-Definition search (digits : list Z) (ts : list (Z -> Z -> Z)) : option Z :=
+Definition search (digits : list Z) (ts : list (Z -> Z -> option Z)) : option Z :=
   let r := memo_fix (length ts) None (_search digits) (0,0%N) ts in
   option_map decimal r.
 
@@ -228,3 +232,196 @@ Definition solve2 (i : list instr) : option Z :=
 Definition solve12 i := (solve i, solve2 i).
 
 (* Compute solve example. *)
+
+Fixpoint compile (xs : list (Z * Z * Z)) : list instr :=
+  match xs with
+  | nil => nil
+  | (A,B,C) :: xs =>
+       `` inp w
+    :: `` mul x 0
+    :: `` add x z
+    :: `` mod x 26
+    :: `` div z (imm A)
+    :: `` add x (imm B)
+    :: `` eql x w
+    :: `` eql x 0
+    :: `` mul y 0
+    :: `` add y 25
+    :: `` mul y x
+    :: `` add y 1
+    :: `` mul z y
+    :: `` mul y 0
+    :: `` add y w
+    :: `` add y (imm C)
+    :: `` mul y x
+    :: `` add z y
+    :: compile xs
+  end.
+
+Ltac destructall :=
+  repeat lazymatch goal with
+  | [ |- context [match ?u with _ => _ end]] => destruct u; try discriminate
+  end.
+
+Lemma compile_recognize xs ys : Some ys = recognize xs -> xs = compile ys.
+Proof.
+  revert xs ys; fix SELF 1; intros [ | x xs] ys; cbn [recognize]; destructall.
+  { injection 1; intros ->; reflexivity. }
+  specialize (SELF xs).
+  destruct (recognize xs) as [ zs | ]; [ | discriminate].
+  specialize (SELF zs eq_refl).
+  cbn [option_map]; injection 1; intros ->.
+  cbn.
+  rewrite SELF. reflexivity.
+Qed.
+
+Lemma recognize_compile xs : Some xs = recognize (compile xs).
+Proof.
+  induction xs as [ | x xs IH ]; [ reflexivity | destruct x as [[A B] C] ]; cbn.
+  rewrite <- IH; reflexivity.
+Qed.
+
+Set Primitive Projections.
+Record regs := Mk_regs
+  { get_w : Z
+  ; get_x : Z
+  ; get_y : Z
+  ; get_z : Z
+  }.
+
+Definition get_reg (r : reg) : regs -> Z :=
+  match r with
+  | imm v => fun _ => v
+  | w => get_w
+  | x => get_x
+  | y => get_y
+  | z => get_z
+  end.
+
+Definition set_reg (r : reg) (v : Z) (rr : regs) : option regs :=
+  let '(Mk_regs rw rx ry rz) := rr in
+  match r with
+  | imm _ => None
+  | w => Some (Mk_regs v rx ry rz)
+  | x => Some (Mk_regs rw v ry rz)
+  | y => Some (Mk_regs rw rx v rz)
+  | z => Some (Mk_regs rw rx ry v)
+  end.
+
+Arguments set_reg r /.
+
+Definition alu_div (x y : Z) : option Z :=
+  if y =? 0 then None else Some (Z.quot x y).
+
+Definition alu_mod (x y : Z) : option Z :=
+  if (x <? 0) || (y <=? 0) then None else Some (Z.modulo x y).
+
+Definition alu_eql (x y : Z) : Z :=
+  if x =? y then 1 else 0.
+
+Definition alu (t : instr) (is : list Z) (rr : regs) : option (list Z * regs) :=
+  let no_input := option_map (fun x => (is, x)) in
+  let evalop (o : Z -> Z -> option Z) :=
+    let r1 := ir1 t in let r2 := ir2 t in
+    mbind (fun v => set_reg r1 v rr) (o (get_reg r1 rr) (get_reg r2 rr)) in
+  let tevalop (o : Z -> Z -> Z) := evalop (fun x y => Some (o x y)) in
+  match iop t with
+  | Add => no_input (tevalop Z.add)
+  | Mul => no_input (tevalop Z.mul)
+  | Div => no_input (evalop alu_div)
+  | Mod => no_input (evalop alu_mod)
+  | Eql => no_input (tevalop alu_eql)
+  | Inp =>
+    match is with
+    | nil => None
+    | v :: is => option_map (fun x => (is, x)) (set_reg (ir1 t) v rr)
+    end
+  end.
+
+Fixpoint alus (ts : list instr) (is : list Z) (rr : regs) : option Z :=
+  match ts with
+  | nil => Some (get_z rr)
+  | t :: ts =>
+    match alu t is rr with
+    | None => None
+    | Some (is, rr) => alus ts is rr
+    end
+  end.
+
+Fixpoint steps (ts : list (Z * Z * Z)) (is : list Z) (rz : Z) : option Z :=
+  match ts, is with
+  | nil, _ => Some rz
+  | t :: ts, i :: is =>
+    match step t i rz with
+    | None => None
+    | Some rz => steps ts is rz
+    end
+  | _ :: _, nil => None
+  end.
+
+Lemma alus_unfold t ts is rr
+  : alus (t :: ts) is rr
+  = match alu t is rr with
+    | None => None
+    | Some (is, rr) => alus ts is rr
+    end.
+Proof. reflexivity. Qed.
+
+Lemma steps_correct ts is rr : steps ts is (get_z rr) = alus (compile ts) is rr.
+Proof.
+  revert is rr; induction ts as [| t ts IH]; cbn; [ reflexivity | intros is rr ].
+  destruct is as [| i is], t as [[A B] C]; [ reflexivity | ].
+  do 4 (rewrite alus_unfold; cbn - [alus]).
+  rewrite Z.mul_0_r, Z.add_0_l.
+  unfold alu_mod. destruct (get_z _ <? 0); [ reflexivity | ].
+  cbn - [alus].
+  do 1 (rewrite alus_unfold; cbn - [alus]).
+  unfold alu_div. destruct (A =? 0); [ reflexivity | ]. cbn - [alus].
+  do 13 (rewrite alus_unfold; cbn - [alus]).
+  rewrite !Z.mul_0_r, !Z.add_0_l.
+  unfold alu_eql. destruct (_ =? _); cbn.
+  { rewrite !Z.mul_0_r, Z.add_0_l, Z.add_0_r, Z.mul_1_r. apply (IH _ (Mk_regs _ _ _ _)). }
+  { rewrite !Z.mul_1_r, Z.add_assoc. apply (IH _ (Mk_regs _ _ _ _)). }
+Qed.
+
+Fixpoint evals (ts : list (Z -> Z -> option Z)) (ws : list Z) (rz : Z) : option Z :=
+  match ts, ws with
+  | t :: ts, rw :: ws =>
+    match t rw rz with
+    | Some rz => evals ts ws rz
+    | None => None
+    end
+  | _ :: _, nil => None
+  | nil, _ => Some rz
+  end.
+
+Lemma evals_steps ts ws rz : evals (map step ts) ws rz = steps ts ws rz.
+Proof.
+  revert ws rz; induction ts as [|t ts IH]; intros; cbn; [ reflexivity | ].
+  destruct ws as [|rw ws]; [ reflexivity | ].
+  destruct step; auto.
+Qed.
+
+Definition smallest {A} (r : relation A) (f : A -> Prop) (x : A) : Prop :=
+  f x /\ (forall y, f y -> r x y).
+
+Definition smallest_lexico {A} `{Lexico A} := smallest (lexico (A := A)).
+Definition greatest_lexico {A} `{Lexico A} := smallest (fun x y : A => lexico y x).
+
+Definition is_digit (x : Z) : Prop := elem_of x (1::2::3::4::5::6::7::8::9::nil).
+
+Theorem solve_correct i ans : solve i = Some ans <->
+  exists i0 res,
+    i = compile i0 /\
+    ans = decimal res /\ Forall is_digit res /\
+    greatest_lexico (fun res' => steps i0 res' 0 = Some 0) res.
+Proof.
+Abort.
+
+Theorem solve2_correct i ans : solve i = Some ans <->
+  exists i0 res,
+    i = compile i0 /\
+    ans = decimal res /\ Forall is_digit res /\
+    smallest_lexico (fun res' => steps i0 res' 0 = Some 0) res.
+Proof.
+Abort.
